\subsection{Example 1}
\begin{figure}[h]
\centerline{
 \scalebox{0.5}{
    \input{../ace/cir1.pstex_t}
 }
}
\end{figure}
\paragraph{First matrices formulation}
X=$^{t}(V_{1},V_{2},V_{3})$\\
\[\left(\begin{array}{c}
  \\
  KCL(1)\\  KCL(2)\\  KCL(3)
  \end{array}\right)
\left(\begin{array}{ccc}
  V_{1}&V_{2}&V_{3}\\
  \hline
  \frac{1}{R}-\frac{1}{R}&  \frac{-1}{R}&0\\
  \frac{1}{R}&  \frac{-1}{R}&0\\
  0&0&\frac{1}{R}
\end{array}\right)X+
\underline{
\left(\begin{array}{ccc}
   V_{1}'&V_{2}'&V_{3}'\\
  \hline
0&0&0\\
  0&C&-C\\
  0&-C&C
\end{array}\right)}X'=
\left(\begin{array}{c}
  \\
  I\\
  0\\
  0
  \end{array}\right)
\]
But, we can't extract x from X to get x'=...\\
\newline
\paragraph{Add current and tension from the capacitor}
x=$(U_{32})$
$Z_{s}=^{t}(V_{1},V_{2},V_{3},I_{32})$\\
\[x'=CI_{32}\]
\[\left(\begin{array}{c}
  \\
  KCL(1)\\
  KCL(2)\\
  KCL(3)\\
  U_{32}
  \end{array}\right)
\left(\begin{array}{cccc}
  V_{1}&V_{2}&V_{3}&I_{32}\\
  \hline
  \frac{1}{R}-\frac{1}{R}&  \frac{-1}{R}&0&0\\
  \frac{1}{R}&  \frac{-1}{R}&0&1\\
  0&0&\frac{1}{R}&-1\\
  0&-1&1&0
\end{array}\right)Z_{s}+
\left(\begin{array}{c}
  U_{32}\\
  \hline
  0\\
  0\\
  0\\
  1
  \end{array}\right)x
=
\left(\begin{array}{c}
  \\
  I\\
  0\\
  0\\
  0
  \end{array}\right)
\]
We obtain the matrices system\\
\[x'=A1_{zs}Z_{s}\]
\[Ax+CZ_{s}=s\]
$N_{I}=N_{E}=5$\\
The following examples, show we don't need to add the capacitor current. Sometime, current in
capacitor can be replace with a KCL law.\\

\paragraph{Add only tension from the capacitor}
x=$(U_{32})$,$Z_{s}=^{t}(V_{1},V_{2},V_{3})$\\
First get x' with \underline{KCL(3)}:
\[x'=\frac{V_{3}}{RC}\]
Second, the current in capacitor is $\frac{V_{3}}{R}$, and use it to write other KCL law:
\[\left(\begin{array}{c}
  \\
  KCL(1)\\
  KCL(2)\\
  U_{32}
  \end{array}\right)
\left(\begin{array}{ccc}
V_{1}&V_{2}&V_{3}\\
  \hline
  \frac{1}{R}+\frac{1}{R}&  \frac{-1}{R}&0\\
  \frac{-1}{R}&  \frac{1}{R}&\frac{1}{R}\\
  0&-1&1
\end{array}\right)Z_{s}+
\left(\begin{array}{c}
U_{32}\\
  \hline
  0\\
  0\\
  0\\
  1
  \end{array}\right)x
=
\left(\begin{array}{c}
  \\
  I\\
  0\\
  0\\
  0
  \end{array}\right)
\]
$N_{I}=N_{E}=4$
\newpage
